{-# OPTIONS --rewriting  #-}

module PR-CC-Ctx where


open import Data.Fin using (Fin; zero; suc)
open import Data.Empty using (âŠ¥)
open import Data.Unit using (âŠ¤; tt)
open import Data.List using (List; [] ; _âˆ·_; _++_; map; concat)
open import Data.Nat using (â„•; suc; zero; _+_)
open import Data.Nat.Properties using (+-suc)
open import Data.Vec using (Vec;[];_âˆ·_;lookup)
open import Data.Product using (_Ã—_; _,_; projâ‚; projâ‚‚) renaming (<_,_> to âŸ¨_,_âŸ©)
open import Data.Sum using (_âŠ_; injâ‚; injâ‚‚)
open import Function using (_âˆ˜_; const) renaming (id to identity)
import Relation.Binary.PropositionalEquality as Eq
open Eq
  using (_â‰¡_; _â‰¢_; refl; sym; trans; cong; congâ‚‚; subst)
open Eq.â‰¡-Reasoning using (begin_; _â‰¡âŸ¨âŸ©_; step-â‰¡Ë˜; step-â‰¡; _âˆ)
open import Utils
open import HVec
open import Agda.Builtin.Equality.Rewrite


import PR-CC-ind as PF


-- infix 6 _â†’á´¾_
infix 7 _`Ã—_
infix 8 _`+_


data Ty n :  Set where
  `ğŸ™   : Ty n
  _`Ã—_ : Ty n â†’ Ty n â†’ Ty n
  _`+_ : Ty n â†’ Ty n â†’ Ty n
  `    : Fin n â†’ Ty n
  ind  : Ty (suc n) â†’ Ty n
  _â‡’_ : Ty n â†’ Ty n â†’ Ty n 

TY = Ty 0



_âŠ¢_â‡’_ : (â„• â†’ Set) â†’ â„• â†’ â„• â†’ Set
_âŠ¢_â‡’_ Trm n m = Fin n â†’ Trm m


record Mappable (Trm : â„• â†’ Set) : Set where
  field â€œ_â€  : âˆ€{n} â†’ Trm n â†’ Ty n
  field ext : âˆ€ {n m} â†’ Trm âŠ¢ n â‡’ m â†’ Trm âŠ¢ (suc n) â‡’ (suc m)
  field ext-cong : âˆ€{n m}{Ïƒ Ï„ : Trm âŠ¢ n â‡’ m} â†’ (âˆ€ (x : Fin n) â†’ Ïƒ x â‰¡ Ï„ x) â†’ (âˆ€(x : Fin (suc n)) â†’ ext {n} Ïƒ x â‰¡ ext {n} Ï„ x)


open Mappable {{...}} public


mapË¢á´¿ : âˆ€ {n m}{Trm}{{_ : Mappable Trm}}
  â†’ (Trm âŠ¢ n â‡’ m)
    -------------------------
  â†’ (Ty n â†’ Ty m)
mapË¢á´¿ f `ğŸ™ = `ğŸ™
mapË¢á´¿ f (tyA `Ã— tyB) = mapË¢á´¿ f tyA `Ã— mapË¢á´¿ f tyB
mapË¢á´¿ f (tyA `+ tyB) = (mapË¢á´¿ f tyA) `+ (mapË¢á´¿ f tyB)
mapË¢á´¿ f (` x) = â€œ (f x) â€
mapË¢á´¿ {n'}{m} f (ind ty) = ind (mapË¢á´¿ (ext {n = n'} f)  ty)
mapË¢á´¿ eq (tyA â‡’ tyB) = mapË¢á´¿ eq tyA â‡’ mapË¢á´¿ eq tyB

map-cong : âˆ€{n m}{T}{{_ : Mappable T}}{Ïƒ Ï„ : T âŠ¢ n â‡’ m}
  â†’ (âˆ€(x : Fin n) â†’ Ïƒ x â‰¡ Ï„ x)
  â†’ âˆ€(ty : Ty n)
  â†’ mapË¢á´¿ Ïƒ ty â‰¡ mapË¢á´¿ Ï„ ty
map-cong eq `ğŸ™ = refl
map-cong {n} {m} {T} eq (tyA `Ã— tyB) = congâ‚‚ _`Ã—_ (map-cong {n} {m} {T} eq tyA) (map-cong {n} {m} {T} eq tyB)
map-cong  {n} {m} {T} eq (tyA `+ tyB) = congâ‚‚ _`+_ (map-cong {n} {m} {T} eq tyA) (map-cong {n} {m} {T} eq tyB)
map-cong eq (` x) = cong â€œ_â€ (eq x)
map-cong eq (ind ty) = cong ind (map-cong (ext-cong eq) ty)
map-cong eq (tyA â‡’ tyB) = congâ‚‚ _â‡’_ (map-cong eq tyA) (map-cong eq tyB)

Ren : â„• â†’ â„• â†’ Set
Ren n m = Fin âŠ¢ n â‡’ m

extá´¿ : âˆ€ {n m} â†’ (Fin âŠ¢ n â‡’ m)
    --------------------------------
  â†’  Fin âŠ¢ (suc n) â‡’ (suc m)
extá´¿ Ï zero      =  zero
extá´¿ Ï (suc x)  =  suc (Ï x)

extá´¿-cong : âˆ€ {n m} {r1 r2 : Ren n m} â†’ (âˆ€ (f : Fin n) â†’ r1 f â‰¡ r2 f) â†’ (âˆ€ (f : Fin (suc n)) â†’ extá´¿ {n} r1 f â‰¡ extá´¿ {n} r2 f )
extá´¿-cong {n} {m} {r1} {r2} eq zero = refl
extá´¿-cong {n} {m} {r1} {r2} eq (suc f) = cong suc (eq f)

instance
  RenameMappable : Mappable Fin
  RenameMappable = record { â€œ_â€ = ` ; ext = extá´¿ ; ext-cong = extá´¿-cong  }


ren : Ren n m â†’ Ty n â†’ Ty m
ren = mapË¢á´¿

Sub : â„• â†’ â„• â†’ Set
Sub n m = Ty âŠ¢ n â‡’ m

extË¢ : âˆ€ {n m} â†’ Sub n m â†’ Sub (suc n) (suc m)
extË¢ Ïƒ zero    = ` zero
extË¢ Ïƒ (suc x) =  mapË¢á´¿  (suc) (Ïƒ x) 


extË¢-cong : âˆ€ {n m} {s1 s2 : Sub n m} â†’ (âˆ€ (f : Fin n) â†’ s1 f â‰¡ s2 f) â†’ (âˆ€ (f : Fin (suc n)) â†’ extË¢ {n} s1 f â‰¡ extË¢ {n} s2 f )
extË¢-cong {n} {m} {s1} {s2} eq zero = refl
extË¢-cong {n} {m} {s1} {s2} eq (suc f) = cong (mapË¢á´¿ suc) (eq f) -- cong (ren suc) (eq f)

instance
  SubstMappable : Mappable Ty
  SubstMappable = record { â€œ_â€ = identity ; ext = extË¢ ; ext-cong = extË¢-cong  }

sub : Sub n m â†’ Ty n â†’ Ty m
sub = mapË¢á´¿ 

idâ‚› : Sub n n
idâ‚› x = ` x

_,â‚›_ : Sub m n â†’ Ty n â†’ Sub (suc m) n
(Ïƒ ,â‚› t) zero    = t
(Ïƒ ,â‚› t) (suc x) = Ïƒ x

Ïƒâ‚€ : Ty n â†’ Sub (suc n) n
Ïƒâ‚€ T = idâ‚› ,â‚› T

subâ‚€ : Ty 0 â†’ Ty 1 â†’ Ty 0
subâ‚€ T       = sub (Ïƒâ‚€ T)


-- record Composable (Tâ‚ Tâ‚‚ Tâ‚ƒ : â„• â†’ Set)
--    {{_ : Mappable Tâ‚}} {{_ : Mappable Tâ‚‚}} {{_ : Mappable Tâ‚ƒ}} : Setâ‚ where
--    infixr 5 _â¨Ÿ_
--    field _â¨Ÿ_ : âˆ€{n m o} â†’ Tâ‚ âŠ¢ n â‡’ m   â†’ Tâ‚‚ âŠ¢ m â‡’ o  â†’  Tâ‚ƒ âŠ¢ n â‡’ o
   
--    field ext-â¨Ÿ : âˆ€{n m o} â†’ (Ïƒâ‚ : Tâ‚ âŠ¢ n â‡’ m) â†’  (Ïƒâ‚‚ : Tâ‚‚ âŠ¢ m â‡’ o) â†’ âˆ€(x : Fin (suc n)) â†’ (ext Ïƒâ‚ â¨Ÿ ext Ïƒâ‚‚) x â‰¡ ext (Ïƒâ‚ â¨Ÿ Ïƒâ‚‚) x
--    field map-â€œâ€ : âˆ€{n m o} â†’ (Ïƒ : Tâ‚ âŠ¢ n â‡’ m) â†’ (Ï„ : Tâ‚‚ âŠ¢ m â‡’ o) â†’ âˆ€(x : Fin n) â†’ mapË¢á´¿ Ï„ â€œ Ïƒ x â€ â‰¡ â€œ (Ïƒ â¨Ÿ Ï„) x â€

-- open Composable {{...}} public

-- -- map-fusionË¢ = {!   !}


-- map-fusion : âˆ€ {n m o}{Tâ‚ Tâ‚‚ Tâ‚ƒ}
--    {{_ : Mappable Tâ‚}}{{_ : Mappable Tâ‚‚}}{{_ : Mappable Tâ‚ƒ}}
--    {{_ : Composable Tâ‚ Tâ‚‚ Tâ‚ƒ}}
--    â†’ (Ïƒ : Tâ‚ âŠ¢ n â‡’ m) â†’ (Ï„ : Tâ‚‚ âŠ¢ m â‡’ o) â†’  (ty : Ty n)
--    â†’ mapË¢á´¿ Ï„ (mapË¢á´¿ Ïƒ ty) â‰¡ mapË¢á´¿ (Ïƒ â¨Ÿ Ï„) ty
-- map-fusion Ïƒ Ï„ `ğŸ™ = refl
-- map-fusion Ïƒ Ï„ (tyA `Ã— tyB) rewrite map-fusion Ïƒ Ï„ tyA  | map-fusion Ïƒ Ï„ tyB = refl
-- map-fusion Ïƒ Ï„ (tyA `+ tyB) rewrite map-fusion Ïƒ Ï„ tyA  | map-fusion Ïƒ Ï„ tyB = refl
-- map-fusion Ïƒ Ï„ (` x) rewrite map-â€œâ€  Ïƒ Ï„ x = refl
-- map-fusion Ïƒ Ï„ (ind ty) rewrite map-fusion (ext Ïƒ) (ext Ï„) ty | map-cong (ext-â¨Ÿ Ïƒ Ï„) ty = cong ind refl



-- _â¨Ÿá´¿_ : âˆ€{n m o} â†’ Fin âŠ¢ n â‡’ m   â†’ Fin âŠ¢ m â‡’ o  â†’  Fin âŠ¢ n â‡’ o
-- (Ïâ‚ â¨Ÿá´¿ Ïâ‚‚) x = Ïâ‚‚ (Ïâ‚ x)



-- -- ```
-- ext-â¨Ÿá´¿ : âˆ€{n m o} (Ïƒ : Fin âŠ¢ n â‡’ m) (Ï„ : Fin âŠ¢ m â‡’ o) â†’ âˆ€ (x : Fin (suc n))
--    â†’ (extá´¿ Ïƒ â¨Ÿá´¿ extá´¿ Ï„) x â‰¡ extá´¿ (Ïƒ â¨Ÿá´¿ Ï„) x
-- ext-â¨Ÿá´¿ {n} {m} {o} Ïƒ Ï„ zero = refl
-- ext-â¨Ÿá´¿ {n} {m} {o} Ïƒ Ï„ (suc x) = refl
-- -- ```

-- -- The `map-â€œâ€` law is trivially proved by the relevant definitions.

-- -- ```
-- instance
--   RenameComposable : Composable Fin Fin Fin
--   RenameComposable = record { _â¨Ÿ_ = _â¨Ÿá´¿_ ; ext-â¨Ÿ = ext-â¨Ÿá´¿ ;
--       map-â€œâ€ = Î» Ïƒ Ï„ x â†’ refl }
-- -- ```

-- -- We obtain a `map-fusion` lemma for renamings, which we name `ren-ren`.

-- -- ```
-- ren-ren : âˆ€ {n m o} â†’ (Ïƒ : Fin âŠ¢ n â‡’ m) â†’ (Ï„ : Fin âŠ¢ m â‡’ o)â†’ âˆ€(ty : Ty n)
--    â†’ ren Ï„ (ren Ïƒ ty) â‰¡ ren (Ïƒ â¨Ÿá´¿ Ï„) ty
-- ren-ren Ïƒ Ï„ ty = map-fusion Ïƒ Ï„ ty
-- -- ```

-- -- ### Substitution and renaming compose into a substitition

-- -- This is also straightforward to prove following the same recipe as
-- -- above.

-- -- ```
-- _á´¿â¨ŸË¢_ : âˆ€{n m o} â†’ Fin âŠ¢ n â‡’ m   â†’ Ty âŠ¢ m â‡’ o  â†’  Ty âŠ¢ n â‡’ o
-- (Ï á´¿â¨ŸË¢ Ïƒ) x = Ïƒ (Ï x)

-- ext-á´¿â¨ŸË¢ : âˆ€{n m o} (Ï : Fin âŠ¢ n â‡’ m) (Ïƒ : Ty âŠ¢ m â‡’ o) â†’ âˆ€(x : Fin (suc n))
--    â†’ (extá´¿ Ï á´¿â¨ŸË¢ extË¢ Ïƒ) x â‰¡ extË¢ (Ï á´¿â¨ŸË¢ Ïƒ) x
-- ext-á´¿â¨ŸË¢ Ï Ïƒ zero = refl
-- ext-á´¿â¨ŸË¢ Ï Ïƒ  (suc x) = refl

-- instance
--   RenameSubstComposable : Composable Fin Ty Ty
--   RenameSubstComposable = record { _â¨Ÿ_ = _á´¿â¨ŸË¢_ ; ext-â¨Ÿ = ext-á´¿â¨ŸË¢ ;
--       map-â€œâ€ = Î» Ïƒ Ï„ x â†’ refl }
-- -- ```

-- -- We obtain a `map-fusion` lemma for a renaming followed by
-- -- a substitution, which we name `ren-sub`.

-- -- ```
-- ren-sub : âˆ€ {n m o} â†’ (Ï : Fin âŠ¢ n â‡’ m) â†’ (Ï„ : Ty âŠ¢ m â‡’ o) â†’ âˆ€ (ty : Ty n)
--    â†’ sub Ï„ (ren Ï ty) â‰¡ sub (Ï á´¿â¨ŸË¢ Ï„) ty
-- ren-sub Ï Ï„ = map-fusion Ï Ï„
-- -- ```

-- -- ### Renaming and substitution compose into a substitution

-- -- The composition of a substitution followed by a renaming
-- -- is defined as follows, using `ren` to apply the renaming
-- -- to the result of `Ïƒ x`.

-- -- ```
-- _Ë¢â¨Ÿá´¿_ : âˆ€{n m o} â†’  Ty âŠ¢ n â‡’ m  â†’  Fin âŠ¢ m â‡’ o  â†’  Ty âŠ¢ n â‡’ o
-- (Ïƒ Ë¢â¨Ÿá´¿ Ï) x = ren Ï (Ïƒ x)
-- -- ```

-- -- The proof of the `ext-â¨Ÿ` law uses the fact that two renamings compose.

-- -- ```
-- ext-Ë¢â¨Ÿá´¿ : âˆ€{n m o} (Ïƒ : Ty âŠ¢ n â‡’ m) (Ï : Fin âŠ¢ m â‡’ o) â†’ âˆ€(x : Fin (suc n))
--    â†’ (extË¢ Ïƒ Ë¢â¨Ÿá´¿ extá´¿ Ï) x â‰¡ extË¢ (Ïƒ Ë¢â¨Ÿá´¿ Ï) x
-- ext-Ë¢â¨Ÿá´¿ Ïƒ Ï zero = refl
-- ext-Ë¢â¨Ÿá´¿ {n}{m} Ïƒ Ï (suc x) =
--   begin
--     (extË¢ Ïƒ Ë¢â¨Ÿá´¿ extá´¿ Ï) (suc x)
--   â‰¡âŸ¨ ren-ren suc (extá´¿ Ï) (Ïƒ x) âŸ©
--     ren (Ï â¨Ÿá´¿ suc) (Ïƒ x)
--   â‰¡âŸ¨ sym (ren-ren Ï suc (Ïƒ x)) âŸ©
--     ren suc ((Ïƒ Ë¢â¨Ÿá´¿ Ï) x)
--   âˆ 
-- -- ```

-- -- The `map-â€œâ€` law is again trivial to prove.

-- -- ```
-- instance
--   SubstRenameComposable : Composable Ty Fin Ty
--   SubstRenameComposable = record { _â¨Ÿ_ = _Ë¢â¨Ÿá´¿_ ;
--       ext-â¨Ÿ = ext-Ë¢â¨Ÿá´¿; map-â€œâ€ = Î» Ïƒ Ï„ x â†’ refl }
-- -- ```

-- -- We obtain a `map-fusion` lemma for a substitution followed by a
-- -- renaming, naming it `sub-ren`.

-- -- ```
-- sub-ren : âˆ€ {n m o} â†’ (Ïƒ : Ty âŠ¢ n â‡’ m) â†’ (Ï : Fin âŠ¢ m â‡’ o) â†’ âˆ€ (ty : Ty n)
--    â†’ ren Ï (sub Ïƒ ty) â‰¡ sub (Ïƒ Ë¢â¨Ÿá´¿ Ï) ty
-- sub-ren Ïƒ Ï = map-fusion Ïƒ Ï
-- -- ```

-- -- ### Two substitutions compose into a substitution

-- -- The composition of two substitutions applies the first substitution to
-- -- the variable, and then applies the second substitution to the
-- -- resulting term using `sub`.

-- -- ```
-- _Ë¢â¨ŸË¢_ : âˆ€{n m o} â†’ Ty âŠ¢ n â‡’ m   â†’ Ty âŠ¢ m â‡’ o  â†’  Ty âŠ¢ n â‡’ o
-- (Ïƒ Ë¢â¨ŸË¢ Ï„) x = sub Ï„ (Ïƒ x)
-- -- ```

-- -- The proof of the `ext-â¨Ÿ` law uses the `ren-sub` and `sub-ren` lemmas.

-- -- ```
-- ext-Ë¢â¨ŸË¢ : âˆ€{n m o} (Ïƒ : Ty âŠ¢ n â‡’ m) (Ï„ : Ty âŠ¢ m â‡’ o)
--    â†’ âˆ€(x : Fin (suc n))
--    â†’ (extË¢ Ïƒ Ë¢â¨ŸË¢ extË¢ Ï„) x â‰¡ extË¢ (Ïƒ Ë¢â¨ŸË¢ Ï„) x
-- ext-Ë¢â¨ŸË¢ Ïƒ Ï„ zero = refl
-- ext-Ë¢â¨ŸË¢ Ïƒ Ï„  (suc x) =
--   begin
--     (extË¢ Ïƒ Ë¢â¨ŸË¢ extË¢ Ï„) (suc x)
--   â‰¡âŸ¨ ren-sub suc (extË¢ Ï„) (Ïƒ x) âŸ©
--     sub (suc á´¿â¨ŸË¢ (extË¢ Ï„)) (Ïƒ x)
--   â‰¡âŸ¨ sym (sub-ren Ï„ suc (Ïƒ x)) âŸ©
--     ren suc ((Ïƒ Ë¢â¨ŸË¢ Ï„) x)
--   âˆ
-- -- ```

-- -- As usual, the `map-â€œâ€` law is trivally true.

-- -- ```
-- instance
--   SubstComposable : Composable Ty Ty Ty
--   SubstComposable = record { _â¨Ÿ_ = _Ë¢â¨ŸË¢_ ; ext-â¨Ÿ = ext-Ë¢â¨ŸË¢ ;
--       map-â€œâ€ = Î» Ïƒ Ï„ x â†’ refl }
-- -- ```

-- -- We obtain a `map-fusion` lemma for the composition of two
-- -- substitutions, naming it `sub-sub`.

-- -- ```
-- sub-sub : âˆ€ {n m o} â†’ (Ïƒ : Ty âŠ¢ n â‡’ m) â†’ (Ï„ : Ty âŠ¢ m â‡’ o) â†’ âˆ€ (ty : Ty n)
--    â†’ sub Ï„ (sub Ïƒ ty) â‰¡ sub (Ïƒ Ë¢â¨ŸË¢ Ï„) ty
-- sub-sub Ïƒ Ï„ = map-fusion Ïƒ Ï„



-- subsub : (Ïƒâ‚ : Sub m o) (Ïƒâ‚‚ : Sub n m) (T : Ty n) â†’ sub Ïƒâ‚ (sub Ïƒâ‚‚ T) â‰¡ sub ((sub Ïƒâ‚) âˆ˜ Ïƒâ‚‚) T
-- subsub Ïƒâ‚ Ïƒâ‚‚ T = sub-sub Ïƒâ‚‚ Ïƒâ‚ T 




variable
  T U V : TY
  G : Ty 1



Ctx : â„• â†’ Set
Ctx n = Vec TY n

data Exp : âˆ€ {n : â„•} â†’ Ctx n â†’ TY â†’ Set where
  `0 :  âˆ€ {n : â„•} {ctx : Ctx n} â†’ Exp ctx ( `ğŸ™)
  App  : âˆ€ {n : â„•} {ctx : Ctx n} {tyA tyB} â†’   Exp ctx (tyA â‡’ tyB) â†’ Exp ctx tyA â†’ Exp ctx tyB
  Var : âˆ€ {n : â„•} {ctx : Ctx n}  â†’ (f : Fin n) â†’ Exp ctx (lookup ctx f)
  Lam  : âˆ€ {n : â„•} {ctx : Ctx n} { tyA tyB} â†’ Exp (tyA âˆ· ctx) tyB â†’ Exp ctx  (tyA â‡’ tyB)


--   --
  `# : âˆ€ {n : â„•} {ctx : Ctx n} { tyA tyB} â†’ Exp ctx tyA â†’ Exp ctx tyB â†’ Exp ctx (tyA `Ã— tyB)
  Ï€â‚ : âˆ€ {n : â„•} {ctx : Ctx n} â†’ Exp ctx (U `Ã— V) â†’ Exp ctx  U
  Ï€â‚‚ : âˆ€ {n : â„•} {ctx : Ctx n} â†’ Exp ctx (U `Ã— V) â†’ Exp ctx  V
--   --
  Î¹â‚ :  âˆ€ {n : â„•} {ctx : Ctx n} â†’  Exp ctx U â†’ Exp ctx (U `+ V)
  Î¹â‚‚ : âˆ€ {n : â„•} {ctx : Ctx n} â†’ Exp ctx V â†’ Exp ctx (U `+ V)
  `case : âˆ€ {n : â„•} {ctx : Ctx n} {tyA tyB tyC : TY} â†’  Exp ctx (tyA `+ tyB) â†’ Exp (tyA âˆ· ctx) (tyC) â†’ Exp (tyB âˆ· ctx) (tyC) â†’ Exp (ctx) (tyC)
--   --
--   fold : subâ‚€ (ind G) G â†’á´¾ ind G
--   P : (h : subâ‚€ (T `Ã— ind G) G `Ã— U â†’á´¾ T) â†’ (ind G `Ã— U â†’á´¾ T)

--   F : (h : subâ‚€ T G `Ã— U â†’á´¾ T) â†’ (ind G `Ã— U â†’á´¾ T)

-- interpretation


âŸ¦_âŸ§áµ€ : TY â†’ Set

data Alg (G : Ty 1) : Set where
  fold : âŸ¦ subâ‚€ (ind G) G âŸ§áµ€ â†’ Alg G 

âŸ¦ `ğŸ™ âŸ§áµ€     = âŠ¤
âŸ¦ T `Ã— U âŸ§áµ€ = âŸ¦ T âŸ§áµ€ Ã— âŸ¦ U âŸ§áµ€
âŸ¦ T `+ U âŸ§áµ€ = âŸ¦ T âŸ§áµ€ âŠ âŸ¦ U âŸ§áµ€
âŸ¦ ind G âŸ§áµ€  = {!   !} -- Alg G
âŸ¦ tyA â‡’ tyB âŸ§áµ€ = âŸ¦ tyA âŸ§áµ€  â†’  âŸ¦ tyB âŸ§áµ€
-- \end{code}
-- }
-- \begin{code}[hide]

-- -- Extensional Function Equality (Homotopies)
-- infix 4 _~_
-- _~_ : âˆ€ {â„“â‚ â„“â‚‚} {A : Set â„“â‚} {B : A â†’ Set â„“â‚‚}
--   â†’ (f g : (x : A) â†’ B x) â†’ Set _
-- f ~ g = âˆ€ x â†’ f x â‰¡ g x 

-- extË¢~ : âˆ€ {m n} {Ïƒâ‚ Ïƒâ‚‚ : Sub m n}
--   â†’ Ïƒâ‚ ~ Ïƒâ‚‚
--   â†’ extË¢ Ïƒâ‚ ~ extË¢ Ïƒâ‚‚
-- extË¢~ Ïƒâ‚~Ïƒâ‚‚ zero = refl
-- extË¢~ Ïƒâ‚~Ïƒâ‚‚ (suc x) = cong (mapË¢á´¿ suc) (Ïƒâ‚~Ïƒâ‚‚ x)

-- sub~ : âˆ€ {m n} {Ïƒâ‚ Ïƒâ‚‚ : Sub m n} {t}
--   â†’ Ïƒâ‚ ~ Ïƒâ‚‚
--   â†’ sub Ïƒâ‚ t â‰¡ sub Ïƒâ‚‚ t
-- sub~ {t = `ğŸ™} f       = refl
-- sub~ {t = tâ‚ `Ã— tâ‚‚} f = congâ‚‚ _`Ã—_ (sub~ {t = tâ‚} f) (sub~ {t = tâ‚‚} f)
-- sub~ {t = tâ‚ `+ tâ‚‚} f = congâ‚‚ _`+_ (sub~ {t = tâ‚} f) (sub~ {t = tâ‚‚} f)
-- sub~ {t = ` x} f      = f x
-- sub~ {t = ind t} f    = cong ind (sub~ {t = t} (extË¢~ f))

-- extË¢-idâ‚› : âˆ€ {n} â†’ extË¢ (idâ‚› {n}) ~ idâ‚›
-- extË¢-idâ‚› zero    = refl
-- extË¢-idâ‚› (suc x) = refl

-- sub-idâ‚› : âˆ€ {n} (t : Ty n) â†’ sub idâ‚› t â‰¡ t
-- sub-idâ‚› `ğŸ™         = refl
-- sub-idâ‚› (tâ‚ `Ã— tâ‚‚) = congâ‚‚ _`Ã—_ (sub-idâ‚› tâ‚) (sub-idâ‚› tâ‚‚)
-- sub-idâ‚› (tâ‚ `+ tâ‚‚) = congâ‚‚ _`+_ (sub-idâ‚› tâ‚) (sub-idâ‚› tâ‚‚)
-- sub-idâ‚› (` x)      = refl
-- sub-idâ‚› (ind t)    = cong ind (trans (sub~ {t = t} extË¢-idâ‚›)
--                                      (sub-idâ‚› t))

-- wk-cancels-,â‚› : âˆ€ {m n} (Ïƒ : Sub m n) T
--     â†’ suc á´¿â¨ŸË¢ (Ïƒ ,â‚› T) ~ Ïƒ
-- wk-cancels-,â‚› Ïƒ T zero    = refl
-- wk-cancels-,â‚› Ïƒ T (suc x) = refl

-- comm-â¨Ÿ-Ïƒâ‚€ : âˆ€ {n m} (Ïƒ : Sub m n) T
--   â†’ (Ïƒâ‚€ T Ë¢â¨ŸË¢ Ïƒ) ~ (extË¢ Ïƒ Ë¢â¨ŸË¢ Ïƒâ‚€ (sub Ïƒ T))
-- comm-â¨Ÿ-Ïƒâ‚€ Ïƒ T zero = refl
-- comm-â¨Ÿ-Ïƒâ‚€ Ïƒ T (suc x) =
--   begin
--     (Ïƒâ‚€ T Ë¢â¨ŸË¢ Ïƒ) (suc x)
--   â‰¡âŸ¨âŸ©
--     Ïƒ x
--   â‰¡âŸ¨ sym (sub-idâ‚› (Ïƒ x)) âŸ©
--     sub idâ‚› (Ïƒ x)
--   â‰¡âŸ¨ sym (sub~ {t = Ïƒ x} (wk-cancels-,â‚› idâ‚› (sub Ïƒ T))) âŸ©
--     sub (suc á´¿â¨ŸË¢ (idâ‚› ,â‚› sub Ïƒ T)) (Ïƒ x)
--   â‰¡âŸ¨ sym (ren-sub suc (idâ‚› ,â‚› sub Ïƒ T) (Ïƒ x)) âŸ©
--     sub (idâ‚› ,â‚› sub Ïƒ T) (ren suc (Ïƒ x))
--   â‰¡âŸ¨âŸ©
--     (extË¢ Ïƒ Ë¢â¨ŸË¢ Ïƒâ‚€ (sub Ïƒ T)) (suc x)
--   âˆ

-- {-# TERMINATING #-}
-- \end{code}
-- \newcommand\ccFunFmap{%
-- \begin{code}
-- fmap : âˆ€ {T} {Gâ‚€ : Ty 1}
--   â†’ (f : âŸ¦ ind Gâ‚€ âŸ§áµ€ â†’ âŸ¦ T âŸ§áµ€) (G : Ty 1)
--   â†’ âŸ¦ subâ‚€ (ind Gâ‚€) G âŸ§áµ€ â†’ âŸ¦ subâ‚€ T G âŸ§áµ€
-- fmap f `ğŸ™ tt = tt
-- fmap f (G `Ã— H) (x , y) = fmap f G x , fmap f H y
-- fmap f (G `+ H) (injâ‚ x) = injâ‚ (fmap f G x)
-- fmap f (G `+ H) (injâ‚‚ y) = injâ‚‚ (fmap f H y)
-- fmap f (` zero) v = f v
-- \end{code}
-- }
-- \begin{code}[hide]
-- fmap {T = T} {Gâ‚€ = Gâ‚€} f (ind G) (fold x) =
--   fold (subst âŸ¦_âŸ§áµ€ (eq (Ïƒâ‚€ T))
--         (fmap{T}{Gâ‚€} f Gâ€²
--          (subst âŸ¦_âŸ§áµ€ (sym (eq (Ïƒâ‚€ (ind Gâ‚€)))) x)))
--   where
--     Gâ€² : Ty 1
--     Gâ€² = sub (Ïƒâ‚€ (ind G)) G
--     eq : âˆ€ (Ï„ : Sub 1 0) â†’ sub Ï„ Gâ€² â‰¡ subâ‚€ (ind (sub (extË¢ Ï„) G)) (sub (extË¢ Ï„) G)
--     eq Ï„ = begin
--        sub Ï„ Gâ€²
--      â‰¡âŸ¨ sub-sub (Ïƒâ‚€ (ind G)) Ï„ G âŸ©
--        sub (Ïƒâ‚€ (ind G) Ë¢â¨ŸË¢ Ï„) G
--      â‰¡âŸ¨ sub~ {t = G} (comm-â¨Ÿ-Ïƒâ‚€ Ï„ (ind G)) âŸ©
--        sub (extË¢ Ï„ Ë¢â¨ŸË¢ Ïƒâ‚€ (sub Ï„ (ind G))) G
--      â‰¡âŸ¨ sym (sub-sub (extË¢ Ï„) (Ïƒâ‚€ (sub Ï„ (ind G))) G) âŸ©
--        subâ‚€ (ind (sub (extË¢ Ï„) G)) (sub (extË¢ Ï„) G)
--      âˆ
-- --- needs to be recursive over `ind G`

-- {-# TERMINATING #-}
-- \end{code}
-- \newcommand\ccFunEval{%
-- \begin{code}
eval : âˆ€ {n : â„•} {ctx : Ctx n} {ty} â†’ Exp ctx ty â†’  HVec (Î» x â†’ âŸ¦ x âŸ§áµ€) ctx â†’ âŸ¦ ty âŸ§áµ€
eval `0 ctx = tt
eval (App f x) ctx = eval f ctx (eval x ctx)
eval (Var f) ctx = hlookup ctx f
eval (Lam exp) ctx = Î» x â†’ eval exp (x âˆ·á´´ ctx)
eval (`# expL expR) ctx = eval expL ctx , eval expR ctx
eval (Ï€â‚ exp) ctx = projâ‚ (eval exp ctx)
eval (Ï€â‚‚ exp) ctx = projâ‚‚ (eval exp ctx)
eval (Î¹â‚ exp) ctx = injâ‚ ((eval exp ctx))
eval (Î¹â‚‚ exp) ctx = injâ‚‚ ((eval exp ctx))
eval (`case exp l r) ctx with eval exp ctx 
... | injâ‚ res = eval l (res âˆ·á´´ ctx)
... | injâ‚‚ res = eval r (res âˆ·á´´ ctx)

embedd-Ty : âˆ€ {n} â†’ PF.Ty n â†’ Ty n
embedd-Ty PF.`ğŸ™ = `ğŸ™
embedd-Ty (tyA PF.`Ã— tyB) = embedd-Ty tyA `Ã— embedd-Ty tyB
embedd-Ty (tyA PF.`+ tyB) = embedd-Ty tyA `+ embedd-Ty tyB
embedd-Ty (PF.` x) = ` x
embedd-Ty (PF.ind ty) = ind (embedd-Ty ty)

weaken : âˆ€ {n : â„•} {ctx : Ctx n} {tyA tyB } â†’  Exp ctx tyA â†’ Exp (tyB âˆ· ctx) tyA
weaken exp = {!   !}



embedd-Exp : âˆ€ {tyA tyB : PF.TY} â†’  tyA PF.â†’á´¾ tyB â†’ Exp [] (embedd-Ty tyA â‡’ embedd-Ty tyB )
embedd-Exp PF.`0 = Lam `0
embedd-Exp PF.id = Lam (Var zero)
embedd-Exp (PF.C f g) = Lam (App (weaken (embedd-Exp f)) (App ((weaken (embedd-Exp g))) (Var zero)))
embedd-Exp (PF.`# l r) = Lam (`# (App (weaken (embedd-Exp l)) (Var zero)) ((App (weaken (embedd-Exp r)) (Var zero))))
embedd-Exp PF.Ï€â‚ = Lam (Ï€â‚ (Var zero))
embedd-Exp PF.Ï€â‚‚ = Lam (Ï€â‚‚ (Var zero))
embedd-Exp PF.Î¹â‚ = Lam (Î¹â‚ ((Var zero)))
embedd-Exp PF.Î¹â‚‚ = Lam (Î¹â‚‚ ((Var zero)))
embedd-Exp (PF.`case f g) = Lam (`case (Var zero) (App (weaken (weaken (embedd-Exp f))) (Var zero)) {!   !})
embedd-Exp PF.fold = {!   !}
embedd-Exp (PF.P exp) = {!   !}
embedd-Exp (PF.F exp) = {!   !}
-- \end{code}
-- }
-- \begin{code}[hide]
-- eval (F {G = G} h) = Î»{ (fold x , u) â†’ eval h ((fmap (Î» v â†’ eval (F h) (v , u)) G x) , u) }
-- \end{code}

-- \begin{code}[hide]
-- mkvec : Ty 0 â†’ â„• â†’ Ty 0
-- mkvec T zero = `ğŸ™
-- mkvec T (suc n) = T `Ã— mkvec T n

-- lookup : (i : Fin n) â†’ mkvec T n â†’á´¾ T
-- lookup zero = Ï€â‚
-- lookup (suc i) = C (lookup i) Ï€â‚‚
-- \end{code}
-- \newcommand\ccFunAssocDist{%
-- \begin{code}
-- assoc-Ã— : (U `Ã— V) `Ã— T â†’á´¾ U `Ã— (V `Ã— T)
-- assoc-Ã— = `# (C Ï€â‚ Ï€â‚) (`# (C Ï€â‚‚ Ï€â‚) Ï€â‚‚)

-- postulate
--   dist-+-x : (U `+ V) `Ã— T â†’á´¾ (U `Ã— T) `+ (V `Ã— T)
-- \end{code}
-- }
-- \begin{code}[hide]
-- module FromNats where
-- \end{code}
-- \newcommand\ccDefGNat{%
-- \begin{code}
--   G-Nat : Ty 1
--   G-Nat = `ğŸ™ `+ ` zero

--   Nat = ind G-Nat

--   _ : subâ‚€ Nat G-Nat â‰¡ (`ğŸ™ `+ Nat)
--   _ = refl

--   -- zero
--   _ : `ğŸ™ â†’á´¾ Nat
--   _ = C fold Î¹â‚

--   _ : `ğŸ™ â†’á´¾ (`ğŸ™ `+ Nat)
--   _ = Î¹â‚

--   -- successor
--   _ : Nat â†’á´¾ Nat
--   _ = C fold Î¹â‚‚

--   _ : Nat â†’á´¾ (`ğŸ™ `+ Nat)
--   _ = Î¹â‚‚
-- \end{code}
-- }
